theories/LambdaWPExamples.v
@@ -1,0 +1,553 @@
+(**
+
+This file defines tactics for manipulating characteristic formula 
+in weakest-precondition form, in lifted Separation Logic,
+as defined in [LambdaWPLifted.v].
+
+Author: Arthur Charguéraud.
+License: MIT.
+
+*)
+
+
+Set Implicit Arguments.
+From Sep Require Export LambdaWPLifted.
+Open Scope heap_scope.
+Generalizable Variables A B.
+
+Implicit Types v w : val.
+Implicit Types t : trm.
+
+Import NotationForVariables NotationForTerms.
+Open Scope val_scope.
+Open Scope pat_scope.
+Open Scope trm_scope.
+
+
+
+(* ********************************************************************** *)
+(* * Demo *)
+
+Ltac hsimpl_wand ::=
+  first [ applys qwand_of_qimpl 
+        | applys hwand_of_himpl ].
+
+
+
+
+(* ---------------------------------------------------------------------- *)
+(** Notation for triples *)
+
+Notation "'TRIPLE' t 'PRE' H 'POST' Q" :=
+  (Triple t H Q)
+  (at level 39, t at level 0) : triple_scope.
+
+Notation "'TRIPLE' t 'PRE' H1 'RET' v 'POST' H2" :=
+  (Triple t H1 (fun r => \[r = v] \* H2))
+  (at level 39, t at level 0) : triple_scope.
+
+Notation "'TRIPLE' t 'PRE' H1 'BIND' x1 'RET' v 'POST' H2" :=
+  (Triple t H1 (fun r => \exists x1, \[r = v] \* H2))
+  (at level 39, t at level 0, x1 ident) : triple_scope.
+
+Notation "'TRIPLE' t 'PRE' H1 'BIND' x1 x2 'RET' v 'POST' H2" :=
+  (Triple t H1 (fun r => \exists x1 x2, \[r = v] \* H2))
+  (at level 39, t at level 0, x1 ident, x2 ident) : triple_scope.
+
+Open Scope triple_scope.
+
+
+(* ---------------------------------------------------------------------- *)
+(* ** Tactic *) 
+
+Lemma Wp_Triple_of_Wp : forall t H `{EA:Enc A} (Q:A->hprop),
+  H ==> ^(Wp Ctx.empty t) Q ->
+  H ==> ^(Wp_Triple t) Q.
+Proof using. introv M. applys himpl_weakestpre. applys* Triple_of_Wp. Qed.
+
+
+
+Lemma Local_erase' : forall H F `{EA:Enc A} (Q:A->hprop),
+  H ==> ^F Q ->
+  H ==> ^(Local F) Q.
+Proof using.
+  introv M. hchanges M. applys local_erase.
+Qed.
+
+(*
+Lemma xlet_lemma : forall Q1 (F1:formula) (F2of:forall `{EA1:Enc A1},A1->Formula) H Q,
+  is_local F1 ->
+  H ==> F1 Q1 ->
+  (forall X, Q1 X ==> F2 X Q) ->
+  H ==> Wp_let F1 F2of Q.
+Proof using.
+  introv L M1 M2. applys local_erase'. applys~ local_weaken M1.
+Qed.
+
+
+
+Definition Wp_let (F1:Formula) (F2of:forall `{EA1:Enc A1},A1->Formula) : Formula :=
+  Local (fun A (EA:Enc A) Q =>
+    \exists (A1:Type) (EA1:Enc A1) ,
+      ^F1 (fun (X:A1) => ^(F2of X) Q)).
+
+*)
+
+(* use:  notypeclasses refine (xlet_instantiate _ _ _). *)
+
+Lemma xlet_instantiate' : forall A1 (EA1:Enc A1) H Fof,
+  H ==> Fof A1 EA1 ->
+  H ==> \exists (A1:Type) (EA1:Enc A1), Fof A1 EA1.
+Proof using. introv M. hsimpl* A1 EA1. Qed.
+
+Lemma xlet_instantiate : forall A1 (EA1:Enc A1) H `{EA:Enc A} (Q:A->hprop) (F1:Formula) (F2of:forall `{EA1:Enc A2},A2->Formula),
+  H ==> ^F1 (fun (X:A1) => ^(F2of X) Q) ->
+  H ==> ^(Wp_let F1 (@F2of)) Q.
+Proof using.
+  introv M. applys Local_erase'. notypeclasses refine (xlet_instantiate' _ _ _). applys M.
+Qed.
+
+(*
+Lemma xlet_typed_instantiate : forall A1 (EA1:Enc A1) H Fof,
+  H ==> Fof A1 EA1 ->
+  H ==> \exists (A1:Type) (EA1:Enc A1), Fof A1 EA1.
+Proof using. introv M. hsimpl* A1 EA1. Qed.
+*)
+
+Lemma xapp_triple_to_Wp_Triple : forall A `{EA:Enc A} (Q1:A->hprop) t H1,
+  Triple t H1 Q1 ->
+  H1 ==> ^(Wp_Triple t) Q1.
+Proof using. introv M. applys* himpl_weakestpre. Qed.
+
+Lemma xapp_lemma' : forall A `{EA:Enc A} (Q1:A->hprop) t H1 H Q,
+  Triple t H1 Q1 ->
+  H ==> H1 \* (Q1 \--* Q) ->
+  H ==> ^(Wp_Triple t) Q.
+Proof using. 
+  introv M1 M2. lets M: xapp_triple_to_Wp_Triple (rm M1).
+  hchanges (rm M2). hchanges (rm M).
+  applys weakestpre_conseq_wand.
+  applys is_local_Triple.
+Qed.
+
+Lemma xapp_lemma : forall A `{EA:Enc A} (Q1:A->hprop) t H1 H Q,
+  Triple t H1 Q1 ->
+  H ==> H1 \* (Q1 \--* Q) ->
+  H ==> ^(Local (Wp_Triple t)) Q.
+Proof using.
+  introv M1 M2. applys Local_erase'. applys* xapp_lemma'.
+Qed.
+
+
+
+Lemma xval_lemma : forall `{EA:Enc A} (V:A) v H (Q:A->hprop),
+  v = ``V ->
+  H ==> Q V ->
+  H ==> ^(Wp_val v) Q.
+Proof using. introv E N. subst. applys Local_erase'. hsimpl~ V. Qed.
+
+Lemma xval_lemma_val : forall `{EA:Enc A} (V:A) v H (Q:val->hprop),
+  v = ``V ->
+  H ==> Q (``V) ->
+  H ==> ^(Wp_val v) Q.
+Proof using. introv E N. subst. applys Local_erase'. hsimpl~ (``V). Qed.
+
+
+
+Lemma xcase_lemma : forall F1 (P:Prop) F2 H `{EA:Enc A} (Q:A->hprop),
+  (H ==> ^F1 Q) ->
+  (P -> H ==> ^F2 Q) ->
+  H ==> ^(Wp_case_val F1 P F2) Q.
+Proof using. 
+  introv M1 M2. apply Local_erase'. applys himpl_hand_r. 
+  { auto. }
+  { applys* hwand_move_l_pure. }
+Qed.
+
+Lemma xcase_lemma0 : forall F1 (P1 P2:Prop) F2 H `{EA:Enc A} (Q:A->hprop),
+  (P1 -> H ==> ^F1 Q) ->
+  (P2 -> H ==> ^F2 Q) ->
+  H ==> ^(Wp_case_val (fun `{EA1:Enc A1} (Q:A1->hprop) => \[P1] \-* ^F1 Q) P2 F2) Q.
+Proof using. 
+  introv M1 M2. applys* xcase_lemma. { applys* hwand_move_l_pure. }
+Qed.
+
+Lemma xcase_lemma2 : forall (F1:val->val->Formula) (P1:val->val->Prop) (P2:Prop) F2 H `{EA:Enc A} (Q:A->hprop),
+  (forall x1 x2, P1 x1 x2 -> H ==> ^(F1 x1 x2) Q) ->
+  (P2 -> H ==> ^F2 Q) ->
+  H ==> ^(Wp_case_val (fun `{EA1:Enc A1} (Q:A1->hprop) => \forall x1 x2, \[P1 x1 x2] \-* ^(F1 x1 x2) Q) P2 F2) Q.
+Proof using. 
+  introv M1 M2. applys* xcase_lemma.
+  { repeat (applys himpl_hforall_r ;=> ?). applys* hwand_move_l_pure. }
+Qed.
+
+Lemma xmatch_list : forall `{EA:Enc A} (L:list A) (F1:Formula) (F2:val->val->Formula) H `{HB:Enc B} (Q:B->hprop),
+  (L = nil -> H ==> ^F1 Q) ->
+  (forall X L', L = X::L' -> H ==> ^(F2 ``X ``L') Q) ->
+  H ==> ^(`Match ``L With
+         '| 'nil '=> F1
+         '| vX ':: vL' [vX vL'] '=> F2 vX vL') Q.
+Proof using.
+  introv M1 M2. applys xcase_lemma0 ;=> E1.
+  { destruct L; rew_enc in *; tryfalse. applys* M1. }
+  { destruct L; rew_enc in *; tryfalse. applys xcase_lemma2.
+    { intros x1 x2 Hx. inverts Hx. applys* M2. }
+    { intros N. false* N. } }
+Qed.
+
+
+
+(* ---------------------------------------------------------------------- *)
+(* ** Lemmas for tactics *)
+
+(*
+Lemma Substn_eq_isubstn : forall xs (Vs:dyns) t,
+  length xs = length Vs ->
+  Substn xs Vs t = isubstn xs (encs Vs) t.
+Proof using.
+  introv E. unfold Substn. rewrite~ isubstn_eq_substn.
+  rewrite* length_encs.
+Qed.
+
+*)
+
+Lemma Triple_apps_funs_of_Wp : forall F (Vs:dyns) (vs:vals) xs t `{EA:Enc A} H (Q:A->hprop),
+  F = val_funs xs t ->
+  vs = encs Vs ->
+  var_funs_exec (length Vs) xs ->
+  H ==> ^(Wp (combine xs (encs Vs)) t) Q ->
+  Triple (trm_apps F vs) H Q.
+Proof using.
+Admitted.
+(*
+  introv EF EV N M. rewrite var_funs_exec_eq in N. rew_istrue in N.
+  subst. applys* Triple_apps_funs. 
+  unfolds in N. rewrite* Substn_eq_isubstn.
+  applys* Triple_isubst_of_Wp.
+Qed.
+*)
+
+Lemma Triple_apps_fixs_of_Wp : forall F (f:var) (Vs:dyns) (vs:vals) xs t `{EA:Enc A} H (Q:A->hprop),
+  F = val_fixs f xs t ->
+  vs = encs Vs ->
+  var_fixs_exec f (length Vs) xs ->
+  H ==> ^(Wp (combine (f::xs) (encs ((Dyn F)::Vs))) t) Q ->
+  Triple (trm_apps F vs) H Q.
+Proof using.
+Admitted.
+(*
+  introv EF EV N M. rewrite var_fixs_exec_eq in N. rew_istrue in N.
+  lets (D&L&_): N. simpl in D. rew_istrue in D. destruct D as [D1 D2].
+  subst. applys* Triple_apps_fixs.
+  rewrite~ Substn_eq_isubstn. 
+  { applys @Triple_isubst_of_Wp M. }
+  { rew_list. math. }
+Qed.
+*)
+
+(* todo: factorize above two using anon? *)
+
+
+Lemma Triple_apps_funs_of_Wp' : forall F (Vs:dyns) (vs:vals) (ts:trms) xs t `{EA:Enc A} H (Q:A->hprop),
+  F = val_funs xs t ->
+  ts = trms_vals vs ->
+  vs = encs Vs ->
+  var_funs_exec (length Vs) xs ->
+  H ==> ^(Wp (combine xs (encs Vs)) t) Q ->
+  Triple (trm_apps F ts) H Q.
+Proof using.
+  intros. subst. applys* Triple_apps_funs_of_Wp.
+Qed.
+(*
+  xcf_prepare_args tt. (* -- not needed here *)
+*)
+
+Lemma Triple_apps_funs_of_Wp'' : forall F (vs:vals) (ts:trms) xs t `{EA:Enc A} H (Q:A->hprop),
+  F = val_funs xs t ->
+  trms_to_vals ts = Some vs ->
+  var_funs_exec (length vs) xs ->
+  H ==> ^(Wp (combine xs vs) t) Q ->
+  Triple (trm_apps F ts) H Q.
+Proof using.
+  introv M1 M2 M3 M4. lets: trms_to_vals_spec M2.
+  skip.
+Qed.
+(*
+  xcf_prepare_args tt. (* -- not needed here *)
+*)
+
+
+
+(* ---------------------------------------------------------------------- *)
+(* * Example proofs *)
+
+Module Test.
+
+
+
+
+(* ---------------------------------------------------------------------- *)
+(* ** Increment *)
+
+Definition val_incr : val :=
+  ValFun 'p :=
+   'p ':= ((val_get 'p) '+ 1).
+
+(* VARIANT:
+  ValFun 'p :=
+    Let 'n := val_get 'p in
+   'p ':= ('n '+ 1).
+*)
+
+
+Lemma triple_incr : forall (p:loc) (n:int),
+  TRIPLE (val_incr ``p)
+    PRE (p ~~> n)
+    POST (fun (r:unit) => (p ~~> (n+1))).
+Proof using.
+  intros.
+  (* xcf details: *)
+  simpl combiner_to_trm.
+  (* xcf_prepare_args tt.  -- not needed here *)
+  (* let f := xcf_get_fun tt in 
+  unfold f. 
+  rew_trms_vals. *)
+  applys Triple_apps_funs_of_Wp''.
+  { reflexivity. }
+  { reflexivity. }
+  { reflexivity. }
+  simpl. rew_enc_dyn. (* xcf_post tt. *)
+  (* fst call *)
+  apply Local_erase'.
+  apply Local_erase'.
+  applys @xapp_lemma. { applys Triple_get. }
+  hsimpl.
+  hsimpl_wand. (* todo: extend hsimpl to do this step *)
+  hpull ;=> ? ->.
+  (* return *)
+  applys @Formula_typed_val. 
+  (* snd call *)
+  applys @xapp_lemma. { eapply @Triple_set. }
+  hsimpl.
+  hsimpl_wand.
+  hsimpl.
+Qed.
+
+(* SHOULD BE:
+
+  xcf.
+  xlet. { xapp. xapplys triple_get. }
+  hpull ;=> ? ->.
+  xlet. { xapp. xapplys triple_add. }
+  hpull ;=> ? ->.
+  xapp. xapplys triple_set. auto.
+
+
+then just:
+
+  xcf.
+  xapp.
+  xapp.
+  xapp.
+
+
+*)
+
+
+
+(* ---------------------------------------------------------------------- *)
+(* ** Case without variables *)
+
+Definition val_test1 : val :=
+  ValFun 'p :=
+    Case' 'p = pat_unit Then 'Fail Else 'Fail.
+
+Lemma triple_test1 : forall (p:loc),
+  TRIPLE (val_test1 ``p)
+    PRE \[]
+    POST (fun (u:unit) => \[]).
+Proof using.
+  intros.
+  (* xcf details: *)
+  simpl combiner_to_trm.
+  applys Triple_apps_funs_of_Wp''; try reflexivity.
+  simpl. rew_enc_dyn.
+Admitted.
+
+
+(* ---------------------------------------------------------------------- *)
+(* ** Case with 1 variable *)
+
+Definition val_test2 : val :=
+  ValFun 'p :=
+    Case' 'p = 'x Then 'x Else 'Fail.
+
+Lemma triple_test2 : forall (p:loc),
+  TRIPLE (val_test2 ``p)
+    PRE \[]
+    POST (fun (u:unit) => \[]).
+Proof using.
+  intros.
+  (* xcf details: *)
+ (* simpl combiner_to_trm.
+  xcf_prepare_args tt. (* -- not needed here *)
+  let f := xcf_get_fun tt in 
+  unfold f.
+  rew_trms_vals. *)
+  applys Triple_apps_funs_of_Wp''; try reflexivity.
+  unfold Ctx.lookup_or_arbitrary. simpl.
+  unfold Wp_var. simpl.
+Admitted.
+
+
+
+(* ---------------------------------------------------------------------- *)
+(* ** Stack *)
+
+(* TODO: is_empty, append *)
+
+Definition val_empty : val :=
+  ValFun 'u :=
+   val_ref 'nil.
+
+Definition val_push : val :=
+  ValFun 'p 'x :=
+   'p ':= ('x ':: (val_get 'p)).
+
+Definition val_pop : val :=
+  ValFun 'p :=
+   (Let 'q := val_get 'p in
+   Match 'q With
+   '| 'nil '=> 'Fail
+   '| 'x ':: 'r '=> ('p ':= 'r) '; 'x
+   End).
+
+Definition Stack `{Enc A} (L:list A) (p:loc) : hprop :=
+  p ~~> L.
+
+
+Lemma triple_pop : forall `{Enc A} (p:loc) (L:list A),
+  L <> nil ->
+  TRIPLE (val_pop ``p)
+    PRE (p ~> Stack L)
+    POST (fun (x:A) => \exists L', \[L = x::L'] \* (p ~> Stack L')).
+Proof using.
+  intros.
+  (* xcf details: 
+  simpl combiner_to_trm.
+  applys Triple_apps_funs_of_Wp'.
+  { reflexivity. }
+  { rew_trms_vals. reflexivity. }
+  { try xeq_encs. }
+  { reflexivity. } *)
+  applys Triple_apps_funs_of_Wp''.
+  { reflexivity. }
+  { reflexivity. }
+  { reflexivity. }
+  simpl; unfold Wp_var.
+  (* start *)
+  xunfold Stack.
+  (* xlet *)
+  notypeclasses refine (xlet_instantiate _ _ _ _ _).
+  (* xapp *)
+  applys @xapp_lemma. { eapply @Triple_get. }
+  hsimpl; hsimpl_wand; hsimpl ;=> ? ->.
+  dup.
+  (* xcase manual *)
+  { applys xcase_lemma0 ;=> E1.
+    { destruct L; tryfalse. }
+    { applys xcase_lemma2.
+      2: { intros E. destruct L; rew_enc in *; tryfalse. }
+      { intros x1 x2 E2. destruct L as [|x L']; rew_enc in *; tryfalse.
+        inverts E2.
+        (* xseq *)
+        (* applys xseq_lemma. *)  apply Local_erase'.
+        (* xapp *)
+        applys @xapp_lemma. { applys @Triple_set. }
+        hsimpl; hsimpl_wand. hsimpl.
+        (* xval *)
+       applys~ xval_lemma.
+        (* post *)
+        hsimpl~. } } }
+  (* xcase with lemma for match list *)
+  { applys xmatch_list.
+    { intros HL. false. }
+    { intros X L' HL. 
+      (* xseq *)
+      (* applys xseq_lemma. *)  apply Local_erase'.
+      (* xapp *)
+      applys @xapp_lemma. { applys @Triple_set. }
+      hsimpl; hsimpl_wand. hsimpl.
+      (* xval *)
+     applys~ xval_lemma.
+      (* post *)
+      hsimpl~. } }
+Qed.
+
+
+
+Lemma triple_empty : forall `{Enc A} (u:unit),
+  TRIPLE (val_empty ``u)
+    PRE \[]
+    POST (fun p => (p ~> Stack (@nil A))).
+Proof using.
+  intros.
+  (* xcf details: *)
+  applys Triple_apps_funs_of_Wp''; try reflexivity.
+  simpl.
+  (* xletval *)
+  apply Local_erase'.
+  (* xval *)
+  applys~ (xval_lemma_val (@nil A)).
+  (* xapp *)
+  applys @xapp_lemma. { eapply @Triple_ref. }
+  hsimpl; hsimpl_wand.
+  hsimpl.
+Qed.
+
+(*
+Definition enc_list `{Enc A} := (fix f (l:list A) :=
+  match l with
+  | nil => val_constr 0%nat nil
+  | x::l' => val_constr 1%nat ((``x)::(f l')::nil)
+  end).
+
+Instance Enc_list2 : forall `{Enc A}, Enc (list A).
+Proof using. constructor. applys enc_list. Defined.
+
+Opaque enc_list.
+*)
+
+Lemma triple_push : forall `{Enc A} (p:loc) (x:A) (L:list A),
+  TRIPLE (val_push ``p ``x)
+    PRE (p ~> Stack L)
+    POST (fun (u:unit) => (p ~> Stack (x::L))).
+Proof using.
+  intros.
+  (* xcf details: *)
+  simpl combiner_to_trm.
+  applys Triple_apps_funs_of_Wp''; try reflexivity. simpl.
+  (* xunfold *)
+  xunfold Stack.
+  (* xval *)
+  apply Local_erase'.
+  (* xlet *)
+  notypeclasses refine (xlet_instantiate _ _ _ _ _).
+  (* xapps *)
+  applys @xapp_lemma. { eapply @Triple_get. }
+  hsimpl. hsimpl_wand. hsimpl ;=> ? ->.
+  (* xval *)
+  applys~ (xval_lemma_val (x::L)).
+  (* xapps *)
+  applys @xapp_lemma. { eapply @Triple_set. }
+  hsimpl. hsimpl_wand. hsimpl ;=> ? ->.
+Qed.
+
+
+
+End Test.
+
+
+
+
+
